QCP_examples/humaneval/spec_logic_rewrite_c_files/C_56_goal.v
@@ -1,0 +1,580 @@
+Require Import Coq.ZArith.ZArith.
+Require Import Coq.Bool.Bool.
+Require Import Coq.Strings.String.
+Require Import Coq.Strings.Ascii.
+Require Import Coq.Lists.List.
+Require Import Coq.Classes.RelationClasses.
+Require Import Coq.Classes.Morphisms.
+Require Import Coq.micromega.Psatz.
+Require Import Coq.Sorting.Permutation.
+From AUXLib Require Import int_auto Axioms Feq Idents ListLib VMap.
+Require Import SetsClass.SetsClass. Import SetsNotation.
+From SimpleC.SL Require Import Mem SeparationLogic.
+Require Import Logic.LogicGenerator.demo932.Interface.
+Local Open Scope Z_scope.
+Local Open Scope sets.
+Local Open Scope string_scope.
+Local Open Scope list.
+Import naive_C_Rules.
+Require Import SimpleC.StdLib.string_lib.
+Require Import coins_56.
+Local Open Scope sac.
+From SimpleC.EE.QCP_demos_LLM Require Import char_array_strategy_goal.
+From SimpleC.EE.QCP_demos_LLM Require Import char_array_strategy_proof.
+From SimpleC.StdLib Require Import string_strategy_goal.
+From SimpleC.StdLib Require Import string_strategy_proof.
+
+(*----- Function correct_bracketing -----*)
+
+Definition correct_bracketing_safety_wit_1 := 
+forall (brackets_pre: Z) (brackets0: Z) (input_l: (@list Z)) (PreH1 : (brackets_pre = brackets0)) (PreH2 : (valid_string input_l )) (PreH3 : (problem_56_pre_z input_l )) (PreH4 : (((string_length (input_l)) + 1 ) < INT_MAX)) ,
+  ((( &( "level" ) )) # Int  |->_)
+  **  ((( &( "brackets" ) )) # Ptr  |-> brackets_pre)
+  **  (store_string brackets_pre input_l )
+|--
+  “ (0 <= INT_MAX) ” 
+  &&  “ ((INT_MIN) <= 0) ”
+.
+
+Definition correct_bracketing_safety_wit_2 := 
+forall (brackets_pre: Z) (brackets0: Z) (input_l: (@list Z)) (retval: Z) (PreH1 : (retval = (string_length (input_l)))) (PreH2 : (0 <= ((string_length (input_l)) + 1 ))) (PreH3 : (brackets_pre = brackets0)) (PreH4 : (valid_string input_l )) (PreH5 : (problem_56_pre_z input_l )) (PreH6 : (((string_length (input_l)) + 1 ) < INT_MAX)) ,
+  ((( &( "i" ) )) # Int  |->_)
+  **  (store_string brackets_pre input_l )
+  **  ((( &( "n" ) )) # Int  |-> retval)
+  **  ((( &( "level" ) )) # Int  |-> 0)
+  **  ((( &( "brackets" ) )) # Ptr  |-> brackets_pre)
+|--
+  “ (0 <= INT_MAX) ” 
+  &&  “ ((INT_MIN) <= 0) ”
+.
+
+Definition correct_bracketing_safety_wit_3 := 
+forall (brackets0: Z) (input_l: (@list Z)) (level: Z) (i: Z) (n: Z) (PreH1 : (i < n)) (PreH2 : (n = (string_length (input_l)))) (PreH3 : (0 <= i)) (PreH4 : (i <= n)) (PreH5 : (0 <= level)) (PreH6 : (level <= i)) (PreH7 : (valid_string input_l )) (PreH8 : (problem_56_pre_z input_l )) (PreH9 : (((string_length (input_l)) + 1 ) < INT_MAX)) (PreH10 : (bracket_state_56 input_l i level )) ,
+  ((( &( "ch" ) )) # Int  |-> (Znth i (c_string (input_l)) 0))
+  **  ((( &( "brackets" ) )) # Ptr  |-> brackets0)
+  **  ((( &( "n" ) )) # Int  |-> n)
+  **  ((( &( "i" ) )) # Int  |-> i)
+  **  ((( &( "level" ) )) # Int  |-> level)
+  **  (store_string brackets0 input_l )
+|--
+  “ (60 <= INT_MAX) ” 
+  &&  “ ((INT_MIN) <= 60) ”
+.
+
+Definition correct_bracketing_safety_wit_4 := 
+forall (brackets0: Z) (input_l: (@list Z)) (level: Z) (i: Z) (n: Z) (PreH1 : ((Znth i (c_string (input_l)) 0) = 60)) (PreH2 : (i < n)) (PreH3 : (n = (string_length (input_l)))) (PreH4 : (0 <= i)) (PreH5 : (i <= n)) (PreH6 : (0 <= level)) (PreH7 : (level <= i)) (PreH8 : (valid_string input_l )) (PreH9 : (problem_56_pre_z input_l )) (PreH10 : (((string_length (input_l)) + 1 ) < INT_MAX)) (PreH11 : (bracket_state_56 input_l i level )) ,
+  ((( &( "ch" ) )) # Int  |-> (Znth i (c_string (input_l)) 0))
+  **  ((( &( "brackets" ) )) # Ptr  |-> brackets0)
+  **  ((( &( "n" ) )) # Int  |-> n)
+  **  ((( &( "i" ) )) # Int  |-> i)
+  **  ((( &( "level" ) )) # Int  |-> level)
+  **  (store_string brackets0 input_l )
+|--
+  “ ((level + 1 ) <= INT_MAX) ” 
+  &&  “ ((INT_MIN) <= (level + 1 )) ”
+.
+
+Definition correct_bracketing_safety_wit_5 := 
+forall (brackets0: Z) (input_l: (@list Z)) (level: Z) (i: Z) (n: Z) (PreH1 : ((Znth i (c_string (input_l)) 0) = 60)) (PreH2 : (i < n)) (PreH3 : (n = (string_length (input_l)))) (PreH4 : (0 <= i)) (PreH5 : (i <= n)) (PreH6 : (0 <= level)) (PreH7 : (level <= i)) (PreH8 : (valid_string input_l )) (PreH9 : (problem_56_pre_z input_l )) (PreH10 : (((string_length (input_l)) + 1 ) < INT_MAX)) (PreH11 : (bracket_state_56 input_l i level )) ,
+  ((( &( "ch" ) )) # Int  |-> (Znth i (c_string (input_l)) 0))
+  **  ((( &( "brackets" ) )) # Ptr  |-> brackets0)
+  **  ((( &( "n" ) )) # Int  |-> n)
+  **  ((( &( "i" ) )) # Int  |-> i)
+  **  ((( &( "level" ) )) # Int  |-> level)
+  **  (store_string brackets0 input_l )
+|--
+  “ (1 <= INT_MAX) ” 
+  &&  “ ((INT_MIN) <= 1) ”
+.
+
+Definition correct_bracketing_safety_wit_6 := 
+forall (brackets0: Z) (input_l: (@list Z)) (level: Z) (i: Z) (n: Z) (PreH1 : ((Znth i (c_string (input_l)) 0) = 60)) (PreH2 : (i < n)) (PreH3 : (n = (string_length (input_l)))) (PreH4 : (0 <= i)) (PreH5 : (i <= n)) (PreH6 : (0 <= level)) (PreH7 : (level <= i)) (PreH8 : (valid_string input_l )) (PreH9 : (problem_56_pre_z input_l )) (PreH10 : (((string_length (input_l)) + 1 ) < INT_MAX)) (PreH11 : (bracket_state_56 input_l i level )) ,
+  ((( &( "ch" ) )) # Int  |-> (Znth i (c_string (input_l)) 0))
+  **  ((( &( "brackets" ) )) # Ptr  |-> brackets0)
+  **  ((( &( "n" ) )) # Int  |-> n)
+  **  ((( &( "i" ) )) # Int  |-> i)
+  **  ((( &( "level" ) )) # Int  |-> (level + 1 ))
+  **  (store_string brackets0 input_l )
+|--
+  “ (62 <= INT_MAX) ” 
+  &&  “ ((INT_MIN) <= 62) ”
+.
+
+Definition correct_bracketing_safety_wit_7 := 
+forall (brackets0: Z) (input_l: (@list Z)) (level: Z) (i: Z) (n: Z) (PreH1 : ((Znth i (c_string (input_l)) 0) <> 60)) (PreH2 : (i < n)) (PreH3 : (n = (string_length (input_l)))) (PreH4 : (0 <= i)) (PreH5 : (i <= n)) (PreH6 : (0 <= level)) (PreH7 : (level <= i)) (PreH8 : (valid_string input_l )) (PreH9 : (problem_56_pre_z input_l )) (PreH10 : (((string_length (input_l)) + 1 ) < INT_MAX)) (PreH11 : (bracket_state_56 input_l i level )) ,
+  ((( &( "ch" ) )) # Int  |-> (Znth i (c_string (input_l)) 0))
+  **  ((( &( "brackets" ) )) # Ptr  |-> brackets0)
+  **  ((( &( "n" ) )) # Int  |-> n)
+  **  ((( &( "i" ) )) # Int  |-> i)
+  **  ((( &( "level" ) )) # Int  |-> level)
+  **  (store_string brackets0 input_l )
+|--
+  “ (62 <= INT_MAX) ” 
+  &&  “ ((INT_MIN) <= 62) ”
+.
+
+Definition correct_bracketing_safety_wit_8 := 
+forall (brackets0: Z) (input_l: (@list Z)) (level: Z) (i: Z) (n: Z) (PreH1 : ((Znth i (c_string (input_l)) 0) = 62)) (PreH2 : ((Znth i (c_string (input_l)) 0) = 60)) (PreH3 : (i < n)) (PreH4 : (n = (string_length (input_l)))) (PreH5 : (0 <= i)) (PreH6 : (i <= n)) (PreH7 : (0 <= level)) (PreH8 : (level <= i)) (PreH9 : (valid_string input_l )) (PreH10 : (problem_56_pre_z input_l )) (PreH11 : (((string_length (input_l)) + 1 ) < INT_MAX)) (PreH12 : (bracket_state_56 input_l i level )) ,
+  ((( &( "ch" ) )) # Int  |-> (Znth i (c_string (input_l)) 0))
+  **  ((( &( "brackets" ) )) # Ptr  |-> brackets0)
+  **  ((( &( "n" ) )) # Int  |-> n)
+  **  ((( &( "i" ) )) # Int  |-> i)
+  **  ((( &( "level" ) )) # Int  |-> (level + 1 ))
+  **  (store_string brackets0 input_l )
+|--
+  “ False ”
+.
+
+Definition correct_bracketing_safety_wit_9 := 
+forall (brackets0: Z) (input_l: (@list Z)) (level: Z) (i: Z) (n: Z) (PreH1 : ((Znth i (c_string (input_l)) 0) = 62)) (PreH2 : ((Znth i (c_string (input_l)) 0) <> 60)) (PreH3 : (i < n)) (PreH4 : (n = (string_length (input_l)))) (PreH5 : (0 <= i)) (PreH6 : (i <= n)) (PreH7 : (0 <= level)) (PreH8 : (level <= i)) (PreH9 : (valid_string input_l )) (PreH10 : (problem_56_pre_z input_l )) (PreH11 : (((string_length (input_l)) + 1 ) < INT_MAX)) (PreH12 : (bracket_state_56 input_l i level )) ,
+  ((( &( "ch" ) )) # Int  |-> (Znth i (c_string (input_l)) 0))
+  **  ((( &( "brackets" ) )) # Ptr  |-> brackets0)
+  **  ((( &( "n" ) )) # Int  |-> n)
+  **  ((( &( "i" ) )) # Int  |-> i)
+  **  ((( &( "level" ) )) # Int  |-> level)
+  **  (store_string brackets0 input_l )
+|--
+  “ ((level - 1 ) <= INT_MAX) ” 
+  &&  “ ((INT_MIN) <= (level - 1 )) ”
+.
+
+Definition correct_bracketing_safety_wit_10 := 
+forall (brackets0: Z) (input_l: (@list Z)) (level: Z) (i: Z) (n: Z) (PreH1 : ((Znth i (c_string (input_l)) 0) = 62)) (PreH2 : ((Znth i (c_string (input_l)) 0) <> 60)) (PreH3 : (i < n)) (PreH4 : (n = (string_length (input_l)))) (PreH5 : (0 <= i)) (PreH6 : (i <= n)) (PreH7 : (0 <= level)) (PreH8 : (level <= i)) (PreH9 : (valid_string input_l )) (PreH10 : (problem_56_pre_z input_l )) (PreH11 : (((string_length (input_l)) + 1 ) < INT_MAX)) (PreH12 : (bracket_state_56 input_l i level )) ,
+  ((( &( "ch" ) )) # Int  |-> (Znth i (c_string (input_l)) 0))
+  **  ((( &( "brackets" ) )) # Ptr  |-> brackets0)
+  **  ((( &( "n" ) )) # Int  |-> n)
+  **  ((( &( "i" ) )) # Int  |-> i)
+  **  ((( &( "level" ) )) # Int  |-> level)
+  **  (store_string brackets0 input_l )
+|--
+  “ (1 <= INT_MAX) ” 
+  &&  “ ((INT_MIN) <= 1) ”
+.
+
+Definition correct_bracketing_safety_wit_11 := 
+forall (brackets0: Z) (input_l: (@list Z)) (level: Z) (i: Z) (n: Z) (PreH1 : ((Znth i (c_string (input_l)) 0) = 62)) (PreH2 : ((Znth i (c_string (input_l)) 0) <> 60)) (PreH3 : (i < n)) (PreH4 : (n = (string_length (input_l)))) (PreH5 : (0 <= i)) (PreH6 : (i <= n)) (PreH7 : (0 <= level)) (PreH8 : (level <= i)) (PreH9 : (valid_string input_l )) (PreH10 : (problem_56_pre_z input_l )) (PreH11 : (((string_length (input_l)) + 1 ) < INT_MAX)) (PreH12 : (bracket_state_56 input_l i level )) ,
+  ((( &( "ch" ) )) # Int  |-> (Znth i (c_string (input_l)) 0))
+  **  ((( &( "brackets" ) )) # Ptr  |-> brackets0)
+  **  ((( &( "n" ) )) # Int  |-> n)
+  **  ((( &( "i" ) )) # Int  |-> i)
+  **  ((( &( "level" ) )) # Int  |-> (level - 1 ))
+  **  (store_string brackets0 input_l )
+|--
+  “ (0 <= INT_MAX) ” 
+  &&  “ ((INT_MIN) <= 0) ”
+.
+
+Definition correct_bracketing_safety_wit_12 := 
+forall (brackets0: Z) (input_l: (@list Z)) (level: Z) (i: Z) (n: Z) (PreH1 : ((Znth i (c_string (input_l)) 0) <> 62)) (PreH2 : ((Znth i (c_string (input_l)) 0) = 60)) (PreH3 : (i < n)) (PreH4 : (n = (string_length (input_l)))) (PreH5 : (0 <= i)) (PreH6 : (i <= n)) (PreH7 : (0 <= level)) (PreH8 : (level <= i)) (PreH9 : (valid_string input_l )) (PreH10 : (problem_56_pre_z input_l )) (PreH11 : (((string_length (input_l)) + 1 ) < INT_MAX)) (PreH12 : (bracket_state_56 input_l i level )) ,
+  ((( &( "ch" ) )) # Int  |-> (Znth i (c_string (input_l)) 0))
+  **  ((( &( "brackets" ) )) # Ptr  |-> brackets0)
+  **  ((( &( "n" ) )) # Int  |-> n)
+  **  ((( &( "i" ) )) # Int  |-> i)
+  **  ((( &( "level" ) )) # Int  |-> (level + 1 ))
+  **  (store_string brackets0 input_l )
+|--
+  “ (0 <= INT_MAX) ” 
+  &&  “ ((INT_MIN) <= 0) ”
+.
+
+Definition correct_bracketing_safety_wit_13 := 
+forall (brackets0: Z) (input_l: (@list Z)) (level: Z) (i: Z) (n: Z) (PreH1 : ((Znth i (c_string (input_l)) 0) <> 62)) (PreH2 : ((Znth i (c_string (input_l)) 0) <> 60)) (PreH3 : (i < n)) (PreH4 : (n = (string_length (input_l)))) (PreH5 : (0 <= i)) (PreH6 : (i <= n)) (PreH7 : (0 <= level)) (PreH8 : (level <= i)) (PreH9 : (valid_string input_l )) (PreH10 : (problem_56_pre_z input_l )) (PreH11 : (((string_length (input_l)) + 1 ) < INT_MAX)) (PreH12 : (bracket_state_56 input_l i level )) ,
+  ((( &( "ch" ) )) # Int  |-> (Znth i (c_string (input_l)) 0))
+  **  ((( &( "brackets" ) )) # Ptr  |-> brackets0)
+  **  ((( &( "n" ) )) # Int  |-> n)
+  **  ((( &( "i" ) )) # Int  |-> i)
+  **  ((( &( "level" ) )) # Int  |-> level)
+  **  (store_string brackets0 input_l )
+|--
+  “ (0 <= INT_MAX) ” 
+  &&  “ ((INT_MIN) <= 0) ”
+.
+
+Definition correct_bracketing_safety_wit_14 := 
+forall (brackets0: Z) (input_l: (@list Z)) (level: Z) (i: Z) (n: Z) (PreH1 : ((level + 1 ) < 0)) (PreH2 : ((Znth i (c_string (input_l)) 0) <> 62)) (PreH3 : ((Znth i (c_string (input_l)) 0) = 60)) (PreH4 : (i < n)) (PreH5 : (n = (string_length (input_l)))) (PreH6 : (0 <= i)) (PreH7 : (i <= n)) (PreH8 : (0 <= level)) (PreH9 : (level <= i)) (PreH10 : (valid_string input_l )) (PreH11 : (problem_56_pre_z input_l )) (PreH12 : (((string_length (input_l)) + 1 ) < INT_MAX)) (PreH13 : (bracket_state_56 input_l i level )) ,
+  ((( &( "ch" ) )) # Int  |-> (Znth i (c_string (input_l)) 0))
+  **  ((( &( "brackets" ) )) # Ptr  |-> brackets0)
+  **  ((( &( "n" ) )) # Int  |-> n)
+  **  ((( &( "i" ) )) # Int  |-> i)
+  **  ((( &( "level" ) )) # Int  |-> (level + 1 ))
+  **  (store_string brackets0 input_l )
+|--
+  “ False ”
+.
+
+Definition correct_bracketing_safety_wit_15 := 
+forall (brackets0: Z) (input_l: (@list Z)) (level: Z) (i: Z) (n: Z) (PreH1 : (level < 0)) (PreH2 : ((Znth i (c_string (input_l)) 0) <> 62)) (PreH3 : ((Znth i (c_string (input_l)) 0) <> 60)) (PreH4 : (i < n)) (PreH5 : (n = (string_length (input_l)))) (PreH6 : (0 <= i)) (PreH7 : (i <= n)) (PreH8 : (0 <= level)) (PreH9 : (level <= i)) (PreH10 : (valid_string input_l )) (PreH11 : (problem_56_pre_z input_l )) (PreH12 : (((string_length (input_l)) + 1 ) < INT_MAX)) (PreH13 : (bracket_state_56 input_l i level )) ,
+  ((( &( "ch" ) )) # Int  |-> (Znth i (c_string (input_l)) 0))
+  **  ((( &( "brackets" ) )) # Ptr  |-> brackets0)
+  **  ((( &( "n" ) )) # Int  |-> n)
+  **  ((( &( "i" ) )) # Int  |-> i)
+  **  ((( &( "level" ) )) # Int  |-> level)
+  **  (store_string brackets0 input_l )
+|--
+  “ False ”
+.
+
+Definition correct_bracketing_safety_wit_16 := 
+forall (brackets0: Z) (input_l: (@list Z)) (level: Z) (i: Z) (n: Z) (PreH1 : ((level - 1 ) < 0)) (PreH2 : ((Znth i (c_string (input_l)) 0) = 62)) (PreH3 : ((Znth i (c_string (input_l)) 0) <> 60)) (PreH4 : (i < n)) (PreH5 : (n = (string_length (input_l)))) (PreH6 : (0 <= i)) (PreH7 : (i <= n)) (PreH8 : (0 <= level)) (PreH9 : (level <= i)) (PreH10 : (valid_string input_l )) (PreH11 : (problem_56_pre_z input_l )) (PreH12 : (((string_length (input_l)) + 1 ) < INT_MAX)) (PreH13 : (bracket_state_56 input_l i level )) ,
+  ((( &( "ch" ) )) # Int  |-> (Znth i (c_string (input_l)) 0))
+  **  ((( &( "brackets" ) )) # Ptr  |-> brackets0)
+  **  ((( &( "n" ) )) # Int  |-> n)
+  **  ((( &( "i" ) )) # Int  |-> i)
+  **  ((( &( "level" ) )) # Int  |-> (level - 1 ))
+  **  (store_string brackets0 input_l )
+|--
+  “ (0 <= INT_MAX) ” 
+  &&  “ ((INT_MIN) <= 0) ”
+.
+
+Definition correct_bracketing_safety_wit_17 := 
+forall (brackets0: Z) (input_l: (@list Z)) (n: Z) (i: Z) (level: Z) (PreH1 : (n = (string_length (input_l)))) (PreH2 : (0 <= i)) (PreH3 : (i < n)) (PreH4 : (0 <= level)) (PreH5 : (level <= (i + 1 ))) (PreH6 : (valid_string input_l )) (PreH7 : (problem_56_pre_z input_l )) (PreH8 : (((string_length (input_l)) + 1 ) < INT_MAX)) (PreH9 : (bracket_state_56 input_l (i + 1 ) level )) ,
+  ((( &( "brackets" ) )) # Ptr  |-> brackets0)
+  **  ((( &( "n" ) )) # Int  |-> n)
+  **  ((( &( "i" ) )) # Int  |-> i)
+  **  ((( &( "level" ) )) # Int  |-> level)
+  **  (store_string brackets0 input_l )
+|--
+  “ ((i + 1 ) <= INT_MAX) ” 
+  &&  “ ((INT_MIN) <= (i + 1 )) ”
+.
+
+Definition correct_bracketing_safety_wit_18 := 
+forall (brackets0: Z) (input_l: (@list Z)) (n: Z) (i: Z) (level: Z) (PreH1 : (n = (string_length (input_l)))) (PreH2 : (0 <= i)) (PreH3 : (i < n)) (PreH4 : (0 <= level)) (PreH5 : (level <= (i + 1 ))) (PreH6 : (valid_string input_l )) (PreH7 : (problem_56_pre_z input_l )) (PreH8 : (((string_length (input_l)) + 1 ) < INT_MAX)) (PreH9 : (bracket_state_56 input_l (i + 1 ) level )) ,
+  ((( &( "brackets" ) )) # Ptr  |-> brackets0)
+  **  ((( &( "n" ) )) # Int  |-> n)
+  **  ((( &( "i" ) )) # Int  |-> i)
+  **  ((( &( "level" ) )) # Int  |-> level)
+  **  (store_string brackets0 input_l )
+|--
+  “ (1 <= INT_MAX) ” 
+  &&  “ ((INT_MIN) <= 1) ”
+.
+
+Definition correct_bracketing_safety_wit_19 := 
+forall (brackets0: Z) (input_l: (@list Z)) (level: Z) (i: Z) (n: Z) (PreH1 : (i >= n)) (PreH2 : (n = (string_length (input_l)))) (PreH3 : (0 <= i)) (PreH4 : (i <= n)) (PreH5 : (0 <= level)) (PreH6 : (level <= i)) (PreH7 : (valid_string input_l )) (PreH8 : (problem_56_pre_z input_l )) (PreH9 : (((string_length (input_l)) + 1 ) < INT_MAX)) (PreH10 : (bracket_state_56 input_l i level )) ,
+  ((( &( "brackets" ) )) # Ptr  |-> brackets0)
+  **  ((( &( "n" ) )) # Int  |-> n)
+  **  ((( &( "i" ) )) # Int  |-> i)
+  **  ((( &( "level" ) )) # Int  |-> level)
+  **  (store_string brackets0 input_l )
+|--
+  “ (0 <= INT_MAX) ” 
+  &&  “ ((INT_MIN) <= 0) ”
+.
+
+Definition correct_bracketing_safety_wit_20 := 
+forall (brackets0: Z) (input_l: (@list Z)) (level: Z) (i: Z) (n: Z) (PreH1 : (level <> 0)) (PreH2 : (i >= n)) (PreH3 : (n = (string_length (input_l)))) (PreH4 : (0 <= i)) (PreH5 : (i <= n)) (PreH6 : (0 <= level)) (PreH7 : (level <= i)) (PreH8 : (valid_string input_l )) (PreH9 : (problem_56_pre_z input_l )) (PreH10 : (((string_length (input_l)) + 1 ) < INT_MAX)) (PreH11 : (bracket_state_56 input_l i level )) ,
+  ((( &( "brackets" ) )) # Ptr  |-> brackets0)
+  **  ((( &( "n" ) )) # Int  |-> n)
+  **  ((( &( "i" ) )) # Int  |-> i)
+  **  ((( &( "level" ) )) # Int  |-> level)
+  **  (store_string brackets0 input_l )
+|--
+  “ (0 <= INT_MAX) ” 
+  &&  “ ((INT_MIN) <= 0) ”
+.
+
+Definition correct_bracketing_safety_wit_21 := 
+forall (brackets0: Z) (input_l: (@list Z)) (level: Z) (i: Z) (n: Z) (PreH1 : (level = 0)) (PreH2 : (i >= n)) (PreH3 : (n = (string_length (input_l)))) (PreH4 : (0 <= i)) (PreH5 : (i <= n)) (PreH6 : (0 <= level)) (PreH7 : (level <= i)) (PreH8 : (valid_string input_l )) (PreH9 : (problem_56_pre_z input_l )) (PreH10 : (((string_length (input_l)) + 1 ) < INT_MAX)) (PreH11 : (bracket_state_56 input_l i level )) ,
+  ((( &( "brackets" ) )) # Ptr  |-> brackets0)
+  **  ((( &( "n" ) )) # Int  |-> n)
+  **  ((( &( "i" ) )) # Int  |-> i)
+  **  ((( &( "level" ) )) # Int  |-> level)
+  **  (store_string brackets0 input_l )
+|--
+  “ (1 <= INT_MAX) ” 
+  &&  “ ((INT_MIN) <= 1) ”
+.
+
+Definition correct_bracketing_entail_wit_1 := 
+(
+forall (brackets_pre: Z) (brackets0: Z) (input_l: (@list Z)) (retval: Z) (PreH1 : (retval = (string_length (input_l)))) (PreH2 : (0 <= ((string_length (input_l)) + 1 ))) (PreH3 : (brackets_pre = brackets0)) (PreH4 : (valid_string input_l )) (PreH5 : (problem_56_pre_z input_l )) (PreH6 : (((string_length (input_l)) + 1 ) < INT_MAX)) ,
+  (store_string brackets_pre input_l )
+  **  ((( &( "brackets" ) )) # Ptr  |-> brackets_pre)
+|--
+  “ (retval = (string_length (input_l))) ” 
+  &&  “ (0 <= 0) ” 
+  &&  “ (0 <= retval) ” 
+  &&  “ (0 <= 0) ” 
+  &&  “ (0 <= 0) ” 
+  &&  “ (valid_string input_l ) ” 
+  &&  “ (problem_56_pre_z input_l ) ” 
+  &&  “ (((string_length (input_l)) + 1 ) < INT_MAX) ” 
+  &&  “ (bracket_state_56 input_l 0 0 ) ”
+  &&  ((( &( "brackets" ) )) # Ptr  |-> brackets0)
+  **  (store_string brackets0 input_l )
+) \/
+(
+forall (brackets_pre: Z) (brackets0: Z) (input_l: (@list Z)) (retval: Z) (PreH1 : (retval = (string_length (input_l)))) (PreH2 : (0 <= ((string_length (input_l)) + 1 ))) (PreH3 : (brackets_pre = brackets0)) (PreH4 : (valid_string input_l )) (PreH5 : (problem_56_pre_z input_l )) (PreH6 : (((string_length (input_l)) + 1 ) < INT_MAX)) ,
+  (CharArray.full brackets_pre ((string_length (input_l)) + 1 ) (c_string (input_l)) )
+|--
+  “ (bracket_state_56 input_l 0 0 ) ” 
+  &&  “ (0 <= retval) ”
+  &&  (CharArray.full brackets0 ((string_length (input_l)) + 1 ) (c_string (input_l)) )
+).
+
+Definition correct_bracketing_entail_wit_1_split_goal_1 := 
+forall (brackets_pre: Z) (brackets0: Z) (input_l: (@list Z)) (retval: Z) (PreH1 : (retval = (string_length (input_l)))) (PreH2 : (0 <= ((string_length (input_l)) + 1 ))) (PreH3 : (brackets_pre = brackets0)) (PreH4 : (valid_string input_l )) (PreH5 : (problem_56_pre_z input_l )) (PreH6 : (((string_length (input_l)) + 1 ) < INT_MAX)) ,
+  (CharArray.full brackets_pre ((string_length (input_l)) + 1 ) (c_string (input_l)) )
+|--
+  “ (bracket_state_56 input_l 0 0 ) ”
+.
+
+Definition correct_bracketing_entail_wit_1_split_goal_2 := 
+forall (brackets_pre: Z) (brackets0: Z) (input_l: (@list Z)) (retval: Z) (PreH1 : (retval = (string_length (input_l)))) (PreH2 : (0 <= ((string_length (input_l)) + 1 ))) (PreH3 : (brackets_pre = brackets0)) (PreH4 : (valid_string input_l )) (PreH5 : (problem_56_pre_z input_l )) (PreH6 : (((string_length (input_l)) + 1 ) < INT_MAX)) ,
+  (CharArray.full brackets_pre ((string_length (input_l)) + 1 ) (c_string (input_l)) )
+|--
+  “ (0 <= retval) ”
+.
+
+Definition correct_bracketing_entail_wit_1_split_goal_spatial := 
+forall (brackets_pre: Z) (brackets0: Z) (input_l: (@list Z)) (retval: Z) (PreH1 : (retval = (string_length (input_l)))) (PreH2 : (0 <= ((string_length (input_l)) + 1 ))) (PreH3 : (brackets_pre = brackets0)) (PreH4 : (valid_string input_l )) (PreH5 : (problem_56_pre_z input_l )) (PreH6 : (((string_length (input_l)) + 1 ) < INT_MAX)) ,
+  (CharArray.full brackets_pre ((string_length (input_l)) + 1 ) (c_string (input_l)) )
+|--
+  (CharArray.full brackets0 ((string_length (input_l)) + 1 ) (c_string (input_l)) )
+.
+
+Definition correct_bracketing_entail_wit_2_1 := 
+(
+forall (brackets0: Z) (input_l: (@list Z)) (level: Z) (i: Z) (n: Z) (PreH1 : (level >= 0)) (PreH2 : ((Znth i (c_string (input_l)) 0) <> 62)) (PreH3 : ((Znth i (c_string (input_l)) 0) <> 60)) (PreH4 : (i < n)) (PreH5 : (n = (string_length (input_l)))) (PreH6 : (0 <= i)) (PreH7 : (i <= n)) (PreH8 : (0 <= level)) (PreH9 : (level <= i)) (PreH10 : (valid_string input_l )) (PreH11 : (problem_56_pre_z input_l )) (PreH12 : (((string_length (input_l)) + 1 ) < INT_MAX)) (PreH13 : (bracket_state_56 input_l i level )) ,
+  (store_string brackets0 input_l )
+|--
+  “ (n = (string_length (input_l))) ” 
+  &&  “ (0 <= i) ” 
+  &&  “ (i < n) ” 
+  &&  “ (0 <= level) ” 
+  &&  “ (level <= (i + 1 )) ” 
+  &&  “ (valid_string input_l ) ” 
+  &&  “ (problem_56_pre_z input_l ) ” 
+  &&  “ (((string_length (input_l)) + 1 ) < INT_MAX) ” 
+  &&  “ (bracket_state_56 input_l (i + 1 ) level ) ”
+  &&  (store_string brackets0 input_l )
+) \/
+(
+forall (input_l: (@list Z)) (level: Z) (i: Z) (n: Z) (PreH1 : (0 <= ((string_length (input_l)) + 1 ))) (PreH2 : (level >= 0)) (PreH3 : ((Znth i (c_string (input_l)) 0) <> 62)) (PreH4 : ((Znth i (c_string (input_l)) 0) <> 60)) (PreH5 : (i < n)) (PreH6 : (n = (string_length (input_l)))) (PreH7 : (0 <= i)) (PreH8 : (i <= n)) (PreH9 : (0 <= level)) (PreH10 : (level <= i)) (PreH11 : (valid_string input_l )) (PreH12 : (problem_56_pre_z input_l )) (PreH13 : (((string_length (input_l)) + 1 ) < INT_MAX)) (PreH14 : (bracket_state_56 input_l i level )) ,
+  TT && emp 
+|--
+  “ (bracket_state_56 input_l (i + 1 ) level ) ”
+  &&  emp
+).
+
+Definition correct_bracketing_entail_wit_2_1_split_goal_1 := 
+forall (input_l: (@list Z)) (level: Z) (i: Z) (n: Z) (PreH1 : (0 <= ((string_length (input_l)) + 1 ))) (PreH2 : (level >= 0)) (PreH3 : ((Znth i (c_string (input_l)) 0) <> 62)) (PreH4 : ((Znth i (c_string (input_l)) 0) <> 60)) (PreH5 : (i < n)) (PreH6 : (n = (string_length (input_l)))) (PreH7 : (0 <= i)) (PreH8 : (i <= n)) (PreH9 : (0 <= level)) (PreH10 : (level <= i)) (PreH11 : (valid_string input_l )) (PreH12 : (problem_56_pre_z input_l )) (PreH13 : (((string_length (input_l)) + 1 ) < INT_MAX)) (PreH14 : (bracket_state_56 input_l i level )) ,
+  TT && emp 
+|--
+  “ (bracket_state_56 input_l (i + 1 ) level ) ”
+.
+
+Definition correct_bracketing_entail_wit_2_2 := 
+(
+forall (brackets0: Z) (input_l: (@list Z)) (level: Z) (i: Z) (n: Z) (PreH1 : ((level + 1 ) >= 0)) (PreH2 : ((Znth i (c_string (input_l)) 0) <> 62)) (PreH3 : ((Znth i (c_string (input_l)) 0) = 60)) (PreH4 : (i < n)) (PreH5 : (n = (string_length (input_l)))) (PreH6 : (0 <= i)) (PreH7 : (i <= n)) (PreH8 : (0 <= level)) (PreH9 : (level <= i)) (PreH10 : (valid_string input_l )) (PreH11 : (problem_56_pre_z input_l )) (PreH12 : (((string_length (input_l)) + 1 ) < INT_MAX)) (PreH13 : (bracket_state_56 input_l i level )) ,
+  (store_string brackets0 input_l )
+|--
+  “ (n = (string_length (input_l))) ” 
+  &&  “ (0 <= i) ” 
+  &&  “ (i < n) ” 
+  &&  “ (0 <= (level + 1 )) ” 
+  &&  “ ((level + 1 ) <= (i + 1 )) ” 
+  &&  “ (valid_string input_l ) ” 
+  &&  “ (problem_56_pre_z input_l ) ” 
+  &&  “ (((string_length (input_l)) + 1 ) < INT_MAX) ” 
+  &&  “ (bracket_state_56 input_l (i + 1 ) (level + 1 ) ) ”
+  &&  (store_string brackets0 input_l )
+) \/
+(
+forall (input_l: (@list Z)) (level: Z) (i: Z) (n: Z) (PreH1 : (0 <= ((string_length (input_l)) + 1 ))) (PreH2 : ((level + 1 ) >= 0)) (PreH3 : ((Znth i (c_string (input_l)) 0) <> 62)) (PreH4 : ((Znth i (c_string (input_l)) 0) = 60)) (PreH5 : (i < n)) (PreH6 : (n = (string_length (input_l)))) (PreH7 : (0 <= i)) (PreH8 : (i <= n)) (PreH9 : (0 <= level)) (PreH10 : (level <= i)) (PreH11 : (valid_string input_l )) (PreH12 : (problem_56_pre_z input_l )) (PreH13 : (((string_length (input_l)) + 1 ) < INT_MAX)) (PreH14 : (bracket_state_56 input_l i level )) ,
+  TT && emp 
+|--
+  “ (bracket_state_56 input_l (i + 1 ) (level + 1 ) ) ”
+  &&  emp
+).
+
+Definition correct_bracketing_entail_wit_2_2_split_goal_1 := 
+forall (input_l: (@list Z)) (level: Z) (i: Z) (n: Z) (PreH1 : (0 <= ((string_length (input_l)) + 1 ))) (PreH2 : ((level + 1 ) >= 0)) (PreH3 : ((Znth i (c_string (input_l)) 0) <> 62)) (PreH4 : ((Znth i (c_string (input_l)) 0) = 60)) (PreH5 : (i < n)) (PreH6 : (n = (string_length (input_l)))) (PreH7 : (0 <= i)) (PreH8 : (i <= n)) (PreH9 : (0 <= level)) (PreH10 : (level <= i)) (PreH11 : (valid_string input_l )) (PreH12 : (problem_56_pre_z input_l )) (PreH13 : (((string_length (input_l)) + 1 ) < INT_MAX)) (PreH14 : (bracket_state_56 input_l i level )) ,
+  TT && emp 
+|--
+  “ (bracket_state_56 input_l (i + 1 ) (level + 1 ) ) ”
+.
+
+Definition correct_bracketing_entail_wit_2_3 := 
+(
+forall (brackets0: Z) (input_l: (@list Z)) (level: Z) (i: Z) (n: Z) (PreH1 : ((level - 1 ) >= 0)) (PreH2 : ((Znth i (c_string (input_l)) 0) = 62)) (PreH3 : ((Znth i (c_string (input_l)) 0) <> 60)) (PreH4 : (i < n)) (PreH5 : (n = (string_length (input_l)))) (PreH6 : (0 <= i)) (PreH7 : (i <= n)) (PreH8 : (0 <= level)) (PreH9 : (level <= i)) (PreH10 : (valid_string input_l )) (PreH11 : (problem_56_pre_z input_l )) (PreH12 : (((string_length (input_l)) + 1 ) < INT_MAX)) (PreH13 : (bracket_state_56 input_l i level )) ,
+  (store_string brackets0 input_l )
+|--
+  “ (n = (string_length (input_l))) ” 
+  &&  “ (0 <= i) ” 
+  &&  “ (i < n) ” 
+  &&  “ (0 <= (level - 1 )) ” 
+  &&  “ ((level - 1 ) <= (i + 1 )) ” 
+  &&  “ (valid_string input_l ) ” 
+  &&  “ (problem_56_pre_z input_l ) ” 
+  &&  “ (((string_length (input_l)) + 1 ) < INT_MAX) ” 
+  &&  “ (bracket_state_56 input_l (i + 1 ) (level - 1 ) ) ”
+  &&  (store_string brackets0 input_l )
+) \/
+(
+forall (input_l: (@list Z)) (level: Z) (i: Z) (n: Z) (PreH1 : (0 <= ((string_length (input_l)) + 1 ))) (PreH2 : ((level - 1 ) >= 0)) (PreH3 : ((Znth i (c_string (input_l)) 0) = 62)) (PreH4 : ((Znth i (c_string (input_l)) 0) <> 60)) (PreH5 : (i < n)) (PreH6 : (n = (string_length (input_l)))) (PreH7 : (0 <= i)) (PreH8 : (i <= n)) (PreH9 : (0 <= level)) (PreH10 : (level <= i)) (PreH11 : (valid_string input_l )) (PreH12 : (problem_56_pre_z input_l )) (PreH13 : (((string_length (input_l)) + 1 ) < INT_MAX)) (PreH14 : (bracket_state_56 input_l i level )) ,
+  TT && emp 
+|--
+  “ (bracket_state_56 input_l (i + 1 ) (level - 1 ) ) ”
+  &&  emp
+).
+
+Definition correct_bracketing_entail_wit_2_3_split_goal_1 := 
+forall (input_l: (@list Z)) (level: Z) (i: Z) (n: Z) (PreH1 : (0 <= ((string_length (input_l)) + 1 ))) (PreH2 : ((level - 1 ) >= 0)) (PreH3 : ((Znth i (c_string (input_l)) 0) = 62)) (PreH4 : ((Znth i (c_string (input_l)) 0) <> 60)) (PreH5 : (i < n)) (PreH6 : (n = (string_length (input_l)))) (PreH7 : (0 <= i)) (PreH8 : (i <= n)) (PreH9 : (0 <= level)) (PreH10 : (level <= i)) (PreH11 : (valid_string input_l )) (PreH12 : (problem_56_pre_z input_l )) (PreH13 : (((string_length (input_l)) + 1 ) < INT_MAX)) (PreH14 : (bracket_state_56 input_l i level )) ,
+  TT && emp 
+|--
+  “ (bracket_state_56 input_l (i + 1 ) (level - 1 ) ) ”
+.
+
+Definition correct_bracketing_entail_wit_3 := 
+forall (brackets0: Z) (input_l: (@list Z)) (n: Z) (i: Z) (level: Z) (PreH1 : (n = (string_length (input_l)))) (PreH2 : (0 <= i)) (PreH3 : (i < n)) (PreH4 : (0 <= level)) (PreH5 : (level <= (i + 1 ))) (PreH6 : (valid_string input_l )) (PreH7 : (problem_56_pre_z input_l )) (PreH8 : (((string_length (input_l)) + 1 ) < INT_MAX)) (PreH9 : (bracket_state_56 input_l (i + 1 ) level )) ,
+  (store_string brackets0 input_l )
+|--
+  “ (n = (string_length (input_l))) ” 
+  &&  “ (0 <= (i + 1 )) ” 
+  &&  “ ((i + 1 ) <= n) ” 
+  &&  “ (0 <= level) ” 
+  &&  “ (level <= (i + 1 )) ” 
+  &&  “ (valid_string input_l ) ” 
+  &&  “ (problem_56_pre_z input_l ) ” 
+  &&  “ (((string_length (input_l)) + 1 ) < INT_MAX) ” 
+  &&  “ (bracket_state_56 input_l (i + 1 ) level ) ”
+  &&  (store_string brackets0 input_l )
+.
+
+Definition correct_bracketing_return_wit_1 := 
+(
+forall (brackets0: Z) (input_l: (@list Z)) (level: Z) (i: Z) (n: Z) (PreH1 : (level = 0)) (PreH2 : (i >= n)) (PreH3 : (n = (string_length (input_l)))) (PreH4 : (0 <= i)) (PreH5 : (i <= n)) (PreH6 : (0 <= level)) (PreH7 : (level <= i)) (PreH8 : (valid_string input_l )) (PreH9 : (problem_56_pre_z input_l )) (PreH10 : (((string_length (input_l)) + 1 ) < INT_MAX)) (PreH11 : (bracket_state_56 input_l i level )) ,
+  (store_string brackets0 input_l )
+|--
+  “ (problem_56_spec_z input_l 1 ) ”
+  &&  (store_string brackets0 input_l )
+) \/
+(
+forall (input_l: (@list Z)) (level: Z) (i: Z) (n: Z) (PreH1 : (0 <= ((string_length (input_l)) + 1 ))) (PreH2 : (level = 0)) (PreH3 : (i >= n)) (PreH4 : (n = (string_length (input_l)))) (PreH5 : (0 <= i)) (PreH6 : (i <= n)) (PreH7 : (0 <= level)) (PreH8 : (level <= i)) (PreH9 : (valid_string input_l )) (PreH10 : (problem_56_pre_z input_l )) (PreH11 : (((string_length (input_l)) + 1 ) < INT_MAX)) (PreH12 : (bracket_state_56 input_l i level )) ,
+  TT && emp 
+|--
+  “ (problem_56_spec_z input_l 1 ) ”
+  &&  emp
+).
+
+Definition correct_bracketing_return_wit_1_split_goal_1 := 
+forall (input_l: (@list Z)) (level: Z) (i: Z) (n: Z) (PreH1 : (0 <= ((string_length (input_l)) + 1 ))) (PreH2 : (level = 0)) (PreH3 : (i >= n)) (PreH4 : (n = (string_length (input_l)))) (PreH5 : (0 <= i)) (PreH6 : (i <= n)) (PreH7 : (0 <= level)) (PreH8 : (level <= i)) (PreH9 : (valid_string input_l )) (PreH10 : (problem_56_pre_z input_l )) (PreH11 : (((string_length (input_l)) + 1 ) < INT_MAX)) (PreH12 : (bracket_state_56 input_l i level )) ,
+  TT && emp 
+|--
+  “ (problem_56_spec_z input_l 1 ) ”
+.
+
+Definition correct_bracketing_return_wit_2 := 
+(
+forall (brackets0: Z) (input_l: (@list Z)) (level: Z) (i: Z) (n: Z) (PreH1 : (level <> 0)) (PreH2 : (i >= n)) (PreH3 : (n = (string_length (input_l)))) (PreH4 : (0 <= i)) (PreH5 : (i <= n)) (PreH6 : (0 <= level)) (PreH7 : (level <= i)) (PreH8 : (valid_string input_l )) (PreH9 : (problem_56_pre_z input_l )) (PreH10 : (((string_length (input_l)) + 1 ) < INT_MAX)) (PreH11 : (bracket_state_56 input_l i level )) ,
+  (store_string brackets0 input_l )
+|--
+  “ (problem_56_spec_z input_l 0 ) ”
+  &&  (store_string brackets0 input_l )
+) \/
+(
+forall (input_l: (@list Z)) (level: Z) (i: Z) (n: Z) (PreH1 : (0 <= ((string_length (input_l)) + 1 ))) (PreH2 : (level <> 0)) (PreH3 : (i >= n)) (PreH4 : (n = (string_length (input_l)))) (PreH5 : (0 <= i)) (PreH6 : (i <= n)) (PreH7 : (0 <= level)) (PreH8 : (level <= i)) (PreH9 : (valid_string input_l )) (PreH10 : (problem_56_pre_z input_l )) (PreH11 : (((string_length (input_l)) + 1 ) < INT_MAX)) (PreH12 : (bracket_state_56 input_l i level )) ,
+  TT && emp 
+|--
+  “ (problem_56_spec_z input_l 0 ) ”
+  &&  emp
+).
+
+Definition correct_bracketing_return_wit_2_split_goal_1 := 
+forall (input_l: (@list Z)) (level: Z) (i: Z) (n: Z) (PreH1 : (0 <= ((string_length (input_l)) + 1 ))) (PreH2 : (level <> 0)) (PreH3 : (i >= n)) (PreH4 : (n = (string_length (input_l)))) (PreH5 : (0 <= i)) (PreH6 : (i <= n)) (PreH7 : (0 <= level)) (PreH8 : (level <= i)) (PreH9 : (valid_string input_l )) (PreH10 : (problem_56_pre_z input_l )) (PreH11 : (((string_length (input_l)) + 1 ) < INT_MAX)) (PreH12 : (bracket_state_56 input_l i level )) ,
+  TT && emp 
+|--
+  “ (problem_56_spec_z input_l 0 ) ”
+.
+
+Definition correct_bracketing_return_wit_3 := 
+(
+forall (brackets0: Z) (input_l: (@list Z)) (level: Z) (i: Z) (n: Z) (PreH1 : ((level - 1 ) < 0)) (PreH2 : ((Znth i (c_string (input_l)) 0) = 62)) (PreH3 : ((Znth i (c_string (input_l)) 0) <> 60)) (PreH4 : (i < n)) (PreH5 : (n = (string_length (input_l)))) (PreH6 : (0 <= i)) (PreH7 : (i <= n)) (PreH8 : (0 <= level)) (PreH9 : (level <= i)) (PreH10 : (valid_string input_l )) (PreH11 : (problem_56_pre_z input_l )) (PreH12 : (((string_length (input_l)) + 1 ) < INT_MAX)) (PreH13 : (bracket_state_56 input_l i level )) ,
+  (store_string brackets0 input_l )
+|--
+  “ (problem_56_spec_z input_l 0 ) ”
+  &&  (store_string brackets0 input_l )
+) \/
+(
+forall (input_l: (@list Z)) (level: Z) (i: Z) (n: Z) (PreH1 : (0 <= ((string_length (input_l)) + 1 ))) (PreH2 : ((level - 1 ) < 0)) (PreH3 : ((Znth i (c_string (input_l)) 0) = 62)) (PreH4 : ((Znth i (c_string (input_l)) 0) <> 60)) (PreH5 : (i < n)) (PreH6 : (n = (string_length (input_l)))) (PreH7 : (0 <= i)) (PreH8 : (i <= n)) (PreH9 : (0 <= level)) (PreH10 : (level <= i)) (PreH11 : (valid_string input_l )) (PreH12 : (problem_56_pre_z input_l )) (PreH13 : (((string_length (input_l)) + 1 ) < INT_MAX)) (PreH14 : (bracket_state_56 input_l i level )) ,
+  TT && emp 
+|--
+  “ (problem_56_spec_z input_l 0 ) ”
+  &&  emp
+).
+
+Definition correct_bracketing_return_wit_3_split_goal_1 := 
+forall (input_l: (@list Z)) (level: Z) (i: Z) (n: Z) (PreH1 : (0 <= ((string_length (input_l)) + 1 ))) (PreH2 : ((level - 1 ) < 0)) (PreH3 : ((Znth i (c_string (input_l)) 0) = 62)) (PreH4 : ((Znth i (c_string (input_l)) 0) <> 60)) (PreH5 : (i < n)) (PreH6 : (n = (string_length (input_l)))) (PreH7 : (0 <= i)) (PreH8 : (i <= n)) (PreH9 : (0 <= level)) (PreH10 : (level <= i)) (PreH11 : (valid_string input_l )) (PreH12 : (problem_56_pre_z input_l )) (PreH13 : (((string_length (input_l)) + 1 ) < INT_MAX)) (PreH14 : (bracket_state_56 input_l i level )) ,
+  TT && emp 
+|--
+  “ (problem_56_spec_z input_l 0 ) ”
+.
+
+Definition correct_bracketing_partial_solve_wit_1_pure := 
+forall (brackets_pre: Z) (brackets0: Z) (input_l: (@list Z)) (PreH1 : (brackets_pre = brackets0)) (PreH2 : (valid_string input_l )) (PreH3 : (problem_56_pre_z input_l )) (PreH4 : (((string_length (input_l)) + 1 ) < INT_MAX)) ,
+  ((( &( "n" ) )) # Int  |->_)
+  **  ((( &( "level" ) )) # Int  |-> 0)
+  **  ((( &( "brackets" ) )) # Ptr  |-> brackets_pre)
+  **  (store_string brackets_pre input_l )
+|--
+  “ (valid_string input_l ) ” 
+  &&  “ ((string_length (input_l)) < INT_MAX) ”
+.
+
+Definition correct_bracketing_partial_solve_wit_1_aux := 
+forall (brackets_pre: Z) (brackets0: Z) (input_l: (@list Z)) (PreH1 : (brackets_pre = brackets0)) (PreH2 : (valid_string input_l )) (PreH3 : (problem_56_pre_z input_l )) (PreH4 : (((string_length (input_l)) + 1 ) < INT_MAX)) ,
+  (store_string brackets_pre input_l )
+|--
+  “ (valid_string input_l ) ” 
+  &&  “ ((string_length (input_l)) < INT_MAX) ” 
+  &&  “ (0 <= ((string_length (input_l)) + 1 )) ” 
+  &&  “ (brackets_pre = brackets0) ” 
+  &&  “ (valid_string input_l ) ” 
+  &&  “ (problem_56_pre_z input_l ) ” 
+  &&  “ (((string_length (input_l)) + 1 ) < INT_MAX) ”
+  &&  (store_string brackets_pre input_l )
+.
+
+Definition correct_bracketing_partial_solve_wit_1 := correct_bracketing_partial_solve_wit_1_pure -> correct_bracketing_partial_solve_wit_1_aux.
+
+Module Type VC_Correct.
+
+Include char_array_Strategy_Correct.
+Include string_Strategy_Correct.
+
+Axiom proof_of_correct_bracketing_safety_wit_1 : correct_bracketing_safety_wit_1.
+Axiom proof_of_correct_bracketing_safety_wit_2 : correct_bracketing_safety_wit_2.
+Axiom proof_of_correct_bracketing_safety_wit_3 : correct_bracketing_safety_wit_3.
+Axiom proof_of_correct_bracketing_safety_wit_4 : correct_bracketing_safety_wit_4.
+Axiom proof_of_correct_bracketing_safety_wit_5 : correct_bracketing_safety_wit_5.
+Axiom proof_of_correct_bracketing_safety_wit_6 : correct_bracketing_safety_wit_6.
+Axiom proof_of_correct_bracketing_safety_wit_7 : correct_bracketing_safety_wit_7.
+Axiom proof_of_correct_bracketing_safety_wit_8 : correct_bracketing_safety_wit_8.
+Axiom proof_of_correct_bracketing_safety_wit_9 : correct_bracketing_safety_wit_9.
+Axiom proof_of_correct_bracketing_safety_wit_10 : correct_bracketing_safety_wit_10.
+Axiom proof_of_correct_bracketing_safety_wit_11 : correct_bracketing_safety_wit_11.
+Axiom proof_of_correct_bracketing_safety_wit_12 : correct_bracketing_safety_wit_12.
+Axiom proof_of_correct_bracketing_safety_wit_13 : correct_bracketing_safety_wit_13.
+Axiom proof_of_correct_bracketing_safety_wit_14 : correct_bracketing_safety_wit_14.
+Axiom proof_of_correct_bracketing_safety_wit_15 : correct_bracketing_safety_wit_15.
+Axiom proof_of_correct_bracketing_safety_wit_16 : correct_bracketing_safety_wit_16.
+Axiom proof_of_correct_bracketing_safety_wit_17 : correct_bracketing_safety_wit_17.
+Axiom proof_of_correct_bracketing_safety_wit_18 : correct_bracketing_safety_wit_18.
+Axiom proof_of_correct_bracketing_safety_wit_19 : correct_bracketing_safety_wit_19.
+Axiom proof_of_correct_bracketing_safety_wit_20 : correct_bracketing_safety_wit_20.
+Axiom proof_of_correct_bracketing_safety_wit_21 : correct_bracketing_safety_wit_21.
+Axiom proof_of_correct_bracketing_entail_wit_1 : correct_bracketing_entail_wit_1.
+Axiom proof_of_correct_bracketing_entail_wit_2_1 : correct_bracketing_entail_wit_2_1.
+Axiom proof_of_correct_bracketing_entail_wit_2_2 : correct_bracketing_entail_wit_2_2.
+Axiom proof_of_correct_bracketing_entail_wit_2_3 : correct_bracketing_entail_wit_2_3.
+Axiom proof_of_correct_bracketing_entail_wit_3 : correct_bracketing_entail_wit_3.
+Axiom proof_of_correct_bracketing_return_wit_1 : correct_bracketing_return_wit_1.
+Axiom proof_of_correct_bracketing_return_wit_2 : correct_bracketing_return_wit_2.
+Axiom proof_of_correct_bracketing_return_wit_3 : correct_bracketing_return_wit_3.
+Axiom proof_of_correct_bracketing_partial_solve_wit_1_pure : correct_bracketing_partial_solve_wit_1_pure.
+Axiom proof_of_correct_bracketing_partial_solve_wit_1 : correct_bracketing_partial_solve_wit_1.
+
+End VC_Correct.
