QCP_examples/humaneval/spec_logic_rewrite_c_files/coins_56.v
@@ -1,0 +1,392 @@
+Load "../spec/56".
+
+Require Import Coq.ZArith.ZArith.
+Require Import Coq.Bool.Bool.
+Require Import Coq.Lists.List.
+Require Import Coq.Strings.Ascii.
+Require Import Coq.Strings.String.
+Require Import Lia.
+From AUXLib Require Import ListLib.
+From SimpleC.SL Require Import IntLib Mem SeparationLogic.
+Require Import SimpleC.StdLib.string_lib.
+
+Import ListNotations.
+Local Open Scope Z_scope.
+Local Open Scope string_scope.
+Local Open Scope list_scope.
+Import naive_C_Rules.
+Local Open Scope sac.
+
+Definition ascii_of_z_56 (z : Z) : ascii :=
+  ascii_of_nat (Z.to_nat z).
+
+Fixpoint string_of_list_z_56 (l : list Z) : string :=
+  match l with
+  | [] => EmptyString
+  | c :: rest => String (ascii_of_z_56 c) (string_of_list_z_56 rest)
+  end.
+
+Definition bool_of_z_56 (z : Z) : bool :=
+  negb (Z.eqb z 0).
+
+Definition problem_56_pre_z (input : list Z) : Prop :=
+  problem_56_pre (string_of_list_z_56 input).
+
+Definition problem_56_spec_z (input : list Z) (result : Z) : Prop :=
+  problem_56_spec (string_of_list_z_56 input) (bool_of_z_56 result).
+
+Inductive BracketScan56 : list Z -> Z -> Prop :=
+| bracket_scan_nil_56 : BracketScan56 [] 0
+| bracket_scan_open_56 : forall prefix depth,
+    BracketScan56 prefix depth ->
+    BracketScan56 (prefix ++ [60]) (depth + 1)
+| bracket_scan_close_56 : forall prefix depth,
+    BracketScan56 prefix depth ->
+    0 < depth ->
+    BracketScan56 (prefix ++ [62]) (depth - 1).
+
+Definition bracket_state_56 (input : list Z) (i level : Z) : Prop :=
+  0 <= i <= Zlength input /\
+  BracketScan56 (firstn (Z.to_nat i) input) level.
+
+Lemma list_ascii_of_string_of_list_z_56 : forall l,
+  list_ascii_of_string (string_of_list_z_56 l) = map ascii_of_z_56 l.
+Proof.
+  induction l as [| c rest IH]; simpl; congruence.
+Qed.
+
+Lemma firstn_succ_snoc_56 : forall {A : Type} n (l : list A) d,
+  (n < List.length l)%nat ->
+  firstn (S n) l = firstn n l ++ [nth n l d].
+Proof.
+  induction n.
+  - intros l d Hn. destruct l; simpl in *; try lia. reflexivity.
+  - intros l d Hn. destruct l; simpl in *; try lia.
+    rewrite (IHn l d) by lia. reflexivity.
+Qed.
+
+Lemma firstn_succ_Znth_56 : forall (l : list Z) i,
+  0 <= i < Zlength l ->
+  firstn (Z.to_nat (i + 1)) l =
+  firstn (Z.to_nat i) l ++ [Znth i l 0].
+Proof.
+  intros l i Hi.
+  replace (Z.to_nat (i + 1)) with (S (Z.to_nat i)) by lia.
+  rewrite firstn_succ_snoc_56 with (d := 0)
+    by (rewrite Zlength_correct in Hi; lia).
+  reflexivity.
+Qed.
+
+Lemma bracket_scan_bounds_56 : forall prefix depth,
+  BracketScan56 prefix depth ->
+  0 <= depth <= Zlength prefix.
+Proof.
+  intros prefix depth Hscan.
+  induction Hscan.
+  - unfold Zlength. simpl. lia.
+  - rewrite Zlength_app. unfold Zlength at 2. simpl. lia.
+  - rewrite Zlength_app. unfold Zlength at 2. simpl. lia.
+Qed.
+
+Lemma bracket_scan_counts_56 : forall prefix depth,
+  BracketScan56 prefix depth ->
+  Z.of_nat (count_occ Z.eq_dec prefix 60) =
+  Z.of_nat (count_occ Z.eq_dec prefix 62) + depth.
+Proof.
+  intros prefix depth Hscan.
+  induction Hscan.
+  - simpl. lia.
+  - rewrite !count_occ_app. simpl. lia.
+  - rewrite !count_occ_app. simpl. lia.
+Qed.
+
+Lemma prefix_of_snoc_56 : forall {A : Type} (l : list A) x p s,
+  l ++ [x] = p ++ s ->
+  (exists t, l = p ++ t) \/ (p = l ++ [x] /\ s = []).
+Proof.
+  intros A l x p s Heq.
+  assert (Hlen : (List.length p <= List.length l + 1)%nat).
+  { apply (f_equal (@List.length A)) in Heq.
+    rewrite !app_length in Heq. simpl in Heq. lia. }
+  destruct (le_gt_dec (List.length p) (List.length l)) as [Hple | Hgt].
+  - left. exists (skipn (List.length p) l).
+    rewrite <- firstn_skipn with (n := List.length p) (l := l) at 1.
+    assert (Hp : firstn (List.length p) l = p).
+    { apply (f_equal (firstn (List.length p))) in Heq.
+      rewrite !firstn_app in Heq.
+      rewrite firstn_all in Heq.
+      replace (List.length p - List.length l)%nat with 0%nat in Heq by lia.
+      replace (List.length p - List.length p)%nat with 0%nat in Heq by lia.
+      simpl in Heq. rewrite !app_nil_r in Heq. exact Heq. }
+    now rewrite Hp.
+  - right.
+    pose proof Heq as HlenEq.
+    apply (f_equal (@List.length A)) in HlenEq.
+    rewrite !app_length in HlenEq. simpl in HlenEq.
+    assert (List.length p = (List.length l + 1)%nat) by lia.
+    assert (List.length s = 0%nat) by lia.
+    apply length_zero_iff_nil in H0. subst s.
+    rewrite app_nil_r in Heq. split; congruence.
+Qed.
+
+Lemma bracket_scan_prefix_ok_56 : forall input depth,
+  BracketScan56 input depth ->
+  forall prefix suffix,
+    input = prefix ++ suffix ->
+    (count_occ Z.eq_dec prefix (62%Z) <=
+     count_occ Z.eq_dec prefix (60%Z))%nat.
+Proof.
+  intros input depth Hscan.
+  induction Hscan as
+      [| input depth Hscan IH | input depth Hscan Hdepth IH];
+    intros prefix suffix Heq.
+  - destruct prefix; simpl in *; try discriminate; lia.
+  - destruct (prefix_of_snoc_56 input 60 prefix suffix Heq)
+      as [[tail Hinput] | [-> ->]].
+    + eapply IH; eauto.
+    + rewrite !count_occ_app. simpl.
+      pose proof (bracket_scan_counts_56 input depth Hscan).
+      pose proof (bracket_scan_bounds_56 input depth Hscan). lia.
+  - destruct (prefix_of_snoc_56 input 62 prefix suffix Heq)
+      as [[tail Hinput] | [-> ->]].
+    + eapply Hdepth; eauto.
+    + rewrite !count_occ_app. simpl.
+      pose proof (bracket_scan_counts_56 input depth Hscan). lia.
+Qed.
+
+Definition angle_code_56 (z : Z) : Prop := z = 60 \/ z = 62.
+
+Lemma bracket_scan_codes_56 : forall input depth,
+  BracketScan56 input depth -> Forall angle_code_56 input.
+Proof.
+  intros input depth Hscan. induction Hscan.
+  - constructor.
+  - apply Forall_app. split; [exact IHHscan |].
+    constructor; [left; reflexivity | constructor].
+  - apply Forall_app. split; [exact IHHscan |].
+    constructor; [right; reflexivity | constructor].
+Qed.
+
+Lemma angle_counts_map_56 : forall input,
+  Forall angle_code_56 input ->
+  count_occ ascii_dec (map ascii_of_z_56 input) "<"%char =
+    count_occ Z.eq_dec input 60 /\
+  count_occ ascii_dec (map ascii_of_z_56 input) ">"%char =
+    count_occ Z.eq_dec input 62.
+Proof.
+  intros input Hcodes. induction Hcodes as [| z input Hz Hcodes IH].
+  - simpl. auto.
+  - destruct Hz as [-> | ->]; simpl in *; destruct IH; split; lia.
+Qed.
+
+Lemma bracket_scan_correctly_56 : forall input,
+  BracketScan56 input 0 ->
+  correctly_bracketed (map ascii_of_z_56 input).
+Proof.
+  intros input Hscan.
+  unfold correctly_bracketed. split.
+  - pose proof (bracket_scan_counts_56 input 0 Hscan) as Hcounts.
+    pose proof (angle_counts_map_56 input
+      (bracket_scan_codes_56 input 0 Hscan)) as [Hopen Hclose].
+    lia.
+  - intros prefix suffix Heq.
+    set (raw_prefix := firstn (List.length prefix) input).
+    set (raw_suffix := skipn (List.length prefix) input).
+    assert (Hraw : input = raw_prefix ++ raw_suffix).
+    { unfold raw_prefix, raw_suffix. symmetry. apply firstn_skipn. }
+    assert (Hprefix : prefix = map ascii_of_z_56 raw_prefix).
+    { apply (f_equal (firstn (List.length prefix))) in Heq.
+      rewrite firstn_map in Heq.
+      rewrite firstn_app in Heq.
+      rewrite firstn_all in Heq.
+      replace (List.length prefix - List.length prefix)%nat with 0%nat in Heq by lia.
+      simpl in Heq. rewrite !app_nil_r in Heq.
+      unfold raw_prefix. symmetry. exact Heq. }
+    pose proof (bracket_scan_prefix_ok_56 input 0 Hscan
+      raw_prefix raw_suffix Hraw) as Hraw_ok.
+    pose proof (bracket_scan_codes_56 input 0 Hscan) as Hall.
+    rewrite Hraw in Hall. apply Forall_app in Hall as [Hprefix_codes _].
+    pose proof (angle_counts_map_56 raw_prefix Hprefix_codes)
+      as [Hopen Hclose].
+    rewrite Hprefix. lia.
+Qed.
+
+Lemma bracket_scan_nonzero_not_correct_56 : forall input depth,
+  BracketScan56 input depth ->
+  depth <> 0 ->
+  ~ correctly_bracketed (map ascii_of_z_56 input).
+Proof.
+  intros input depth Hscan Hdepth [Heq _].
+  pose proof (bracket_scan_counts_56 input depth Hscan) as Hcounts.
+  pose proof (angle_counts_map_56 input
+    (bracket_scan_codes_56 input depth Hscan)) as [Hopen Hclose].
+  lia.
+Qed.
+
+Lemma ascii_of_z_angle_raw_56 : forall z,
+  0 <= z <= 127 ->
+  (ascii_of_z_56 z = "<"%char \/ ascii_of_z_56 z = ">"%char) ->
+  z = 60 \/ z = 62.
+Proof.
+  intros z Hz [Hchar | Hchar].
+  - left. apply (f_equal nat_of_ascii) in Hchar.
+    unfold ascii_of_z_56 in Hchar.
+    rewrite nat_ascii_embedding in Hchar by lia.
+    cbn in Hchar. lia.
+  - right. apply (f_equal nat_of_ascii) in Hchar.
+    unfold ascii_of_z_56 in Hchar.
+    rewrite nat_ascii_embedding in Hchar by lia.
+    cbn in Hchar. lia.
+Qed.
+
+Lemma problem_56_pre_code_at : forall input i,
+  problem_56_pre_z input ->
+  string_lib.valid_string input ->
+  0 <= i < string_lib.string_length input ->
+  Znth i input 0 = 60 \/ Znth i input 0 = 62.
+Proof.
+  intros input i Hpre Hvalid Hi.
+  unfold problem_56_pre_z, problem_56_pre in Hpre.
+  rewrite list_ascii_of_string_of_list_z_56 in Hpre.
+  assert (Hin : In (Znth i input 0) input).
+  { unfold Znth.
+    apply nth_In.
+    unfold string_lib.string_length in Hi.
+    rewrite Zlength_correct in Hi. lia. }
+  assert (Hascii :
+      ascii_of_z_56 (Znth i input 0) = "<"%char \/
+      ascii_of_z_56 (Znth i input 0) = ">"%char).
+  { rewrite Forall_forall in Hpre. apply Hpre.
+    apply in_map. exact Hin. }
+  apply ascii_of_z_angle_raw_56; [|exact Hascii].
+  unfold string_lib.valid_string, string_lib.all_ascii in Hvalid.
+  destruct Hvalid as [Hrange _]. apply Hrange. exact Hi.
+Qed.
+
+Lemma bracket_state_full_scan_56 : forall input i depth,
+  bracket_state_56 input i depth ->
+  i >= string_lib.string_length input ->
+  BracketScan56 input depth.
+Proof.
+  intros input i depth [[Hi0 Hiend] Hscan] Hdone.
+  unfold string_lib.string_length in Hdone.
+  assert (i = Zlength input) by lia. subst i.
+  replace (Z.to_nat (Zlength input)) with (List.length input) in Hscan.
+  - now rewrite firstn_all in Hscan.
+  - rewrite Zlength_correct. lia.
+Qed.
+
+Lemma bracket_state_zero_spec_56 : forall input i,
+  bracket_state_56 input i 0 ->
+  i >= string_lib.string_length input ->
+  problem_56_spec_z input 1.
+Proof.
+  intros input i Hstate Hdone.
+  pose proof (bracket_state_full_scan_56 input i 0 Hstate Hdone) as Hscan.
+  unfold problem_56_spec_z, bool_of_z_56, problem_56_spec. simpl.
+  rewrite list_ascii_of_string_of_list_z_56.
+  split; [intro; apply bracket_scan_correctly_56; exact Hscan | auto].
+Qed.
+
+Lemma bracket_state_nonzero_spec_56 : forall input i depth,
+  bracket_state_56 input i depth ->
+  i >= string_lib.string_length input ->
+  depth <> 0 ->
+  problem_56_spec_z input 0.
+Proof.
+  intros input i depth Hstate Hdone Hdepth.
+  pose proof (bracket_state_full_scan_56 input i depth Hstate Hdone) as Hscan.
+  unfold problem_56_spec_z, bool_of_z_56, problem_56_spec. simpl.
+  rewrite list_ascii_of_string_of_list_z_56.
+  split; [discriminate |].
+  intro Hcorrect. exfalso.
+  eapply bracket_scan_nonzero_not_correct_56; eauto.
+Qed.
+
+Lemma bracket_scan_zero_close_bad_56 : forall prefix suffix,
+  BracketScan56 prefix 0 ->
+  ~ correctly_bracketed
+      (map ascii_of_z_56 (prefix ++ [62] ++ suffix)).
+Proof.
+  intros prefix suffix Hscan [_ Hprefix].
+  specialize (Hprefix
+    (map ascii_of_z_56 (prefix ++ [62]))
+    (map ascii_of_z_56 suffix)).
+  assert (Hineq :
+      (count_occ ascii_dec (map ascii_of_z_56 (prefix ++ [62%Z])) ">"%char <=
+       count_occ ascii_dec (map ascii_of_z_56 (prefix ++ [62%Z])) "<"%char)%nat).
+  { apply Hprefix. rewrite !map_app. apply app_assoc. }
+  pose proof (bracket_scan_counts_56 prefix 0 Hscan) as Hcounts.
+  pose proof (angle_counts_map_56 prefix
+    (bracket_scan_codes_56 prefix 0 Hscan)) as [Hopen Hclose].
+  rewrite !map_app in Hineq. simpl in Hineq.
+  rewrite !count_occ_app in Hineq. simpl in Hineq. lia.
+Qed.
+
+Lemma bracket_state_negative_spec_56 : forall input i,
+  bracket_state_56 input i 0 ->
+  0 <= i < string_lib.string_length input ->
+  Znth i input 0 = 62 ->
+  problem_56_spec_z input 0.
+Proof.
+  intros input i [[Hi0 Hiend] Hscan] Hib Hchar.
+  unfold problem_56_spec_z, bool_of_z_56, problem_56_spec. simpl.
+  rewrite list_ascii_of_string_of_list_z_56.
+  split; [discriminate |]. intro Hcorrect. exfalso.
+  unfold string_lib.string_length in Hib.
+  assert (Hnext :
+      firstn (Z.to_nat (i + 1)) input =
+      firstn (Z.to_nat i) input ++ [62]).
+  { rewrite firstn_succ_Znth_56 by exact Hib. now rewrite Hchar. }
+  assert (Hdecomp : input =
+      (firstn (Z.to_nat i) input ++ [62]) ++
+      skipn (Z.to_nat (i + 1)) input).
+  { rewrite <- Hnext. symmetry. apply firstn_skipn. }
+  rewrite Hdecomp in Hcorrect.
+  pose proof (bracket_scan_zero_close_bad_56
+    (firstn (Z.to_nat i) input)
+    (skipn (Z.to_nat (i + 1)) input) Hscan) as Hbad.
+  apply Hbad. rewrite app_assoc. exact Hcorrect.
+Qed.
+
+Lemma bracket_state_nil_56 : forall input,
+  bracket_state_56 input 0 0.
+Proof.
+  intro input. split.
+  - pose proof (Zlength_nonneg input). lia.
+  - simpl. constructor.
+Qed.
+
+Lemma bracket_state_open_56 : forall input i depth,
+  bracket_state_56 input i depth ->
+  0 <= i < Zlength input ->
+  Znth i input 0 = 60 ->
+  bracket_state_56 input (i + 1) (depth + 1).
+Proof.
+  intros input i depth [Hi Hscan] Hib Hchar.
+  split; [lia |].
+  rewrite firstn_succ_Znth_56 by exact Hib.
+  rewrite Hchar. now constructor.
+Qed.
+
+Lemma bracket_state_close_56 : forall input i depth,
+  bracket_state_56 input i depth ->
+  0 <= i < Zlength input ->
+  Znth i input 0 = 62 ->
+  0 < depth ->
+  bracket_state_56 input (i + 1) (depth - 1).
+Proof.
+  intros input i depth [Hi Hscan] Hib Hchar Hdepth.
+  split; [lia |].
+  rewrite firstn_succ_Znth_56 by exact Hib.
+  rewrite Hchar. now constructor.
+Qed.
+
+Lemma Znth_c_string_56 : forall input i,
+  0 <= i < string_lib.string_length input ->
+  Znth i (string_lib.c_string input) 0 = Znth i input 0.
+Proof.
+  intros input i Hi.
+  unfold string_lib.c_string, string_lib.string_length in *.
+  apply app_Znth1. exact Hi.
+Qed.
